feat: move general defs and theorems from DFA to DA

Cslib/Computability/Automata/DA.lean
@@ -4,6 +4,8 @@ Released under Apache 2.0 license as described in the file LICENSE.
 Authors: Fabrizio Montesi
 -/
 
+import Cslib.Foundations.Semantics.LTS.Basic
+
 /-! # Deterministic Automaton
 
 A Deterministic Automaton (DA) is a deterministic labelled transition system with an initial state.
@@ -14,3 +16,57 @@ structure DA (State : Type _) (Symbol : Type _) where
   start : State
   /-- The transition function of the automaton. -/
   tr : State → Symbol → State
+
+namespace DA
+
+/-- Extended transition function.
+
+Implementation note: compared to [Hopcroft2006], the definition consumes the input list of symbols
+from the left (instead of the right), in order to follow the way lists are constructed.
+-/
+@[grind]
+def mtr (da : DA State Symbol) (s : State) (xs : List Symbol) :=
+  match xs with
+  | [] => s
+  | x :: xs => da.mtr (da.tr s x) xs
+
+@[grind]
+theorem mtr_nil_eq {da : DA State Symbol} : da.mtr s [] = s := by rfl
+
+section LTS
+
+/-- `DA` is a special case of `LTS`. -/
+@[grind]
+def toLTS (da : DA State Symbol) : LTS State Symbol :=
+  LTS.mk (fun s1 μ s2 => da.tr s1 μ = s2)
+
+instance : Coe (DA State Symbol) (LTS State Symbol) where
+  coe := toLTS
+
+/-- `DA.toLTS` correctly characterises transitions. -/
+@[grind]
+theorem toLTS_tr {da : DA State Symbol} :
+  da.toLTS.Tr s1 μ s2 ↔ da.tr s1 μ = s2 := by
+  rfl
+
+/-- `DA.toLTS` correctly characterises multistep transitions. -/
+@[grind]
+theorem toLTS_mtr {da : DA State Symbol} :
+  da.toLTS.MTr s1 xs s2 ↔ da.mtr s1 xs = s2 := by
+  constructor <;> intro h
+  case mp =>
+    induction h <;> grind
+  case mpr =>
+    induction xs generalizing s1
+    case nil => grind
+    case cons x xs ih =>
+      apply LTS.MTr.stepL (s2 := da.tr s1 x) <;> grind
+
+/-- The LTS induced by a DA is deterministic. -/
+@[grind]
+theorem toLTS_deterministic (da : DA State Symbol) : da.toLTS.Deterministic := by
+  grind
+
+end LTS
+
+end DA
